p256: add fsti for LowLevel

code/ecdsap256/Hacl.Impl.P256.LowLevel.fst
@@ -16,44 +16,40 @@ module SN = Hacl.Spec.Bignum
 
 #set-options "--z3rlimit 50 --fuel 0 --ifuel 0"
 
-inline_for_extraction noextract
-val mul: f:felem -> r:felem -> out:widefelem -> Stack unit
-  (requires fun h ->
-    live h out /\ live h f /\ live h r /\
-    eq_or_disjoint r f /\ disjoint f out /\ disjoint r out)
-  (ensures  fun h0 _ h1 -> modifies (loc out) h0 h1 /\
-    wide_as_nat h1 out = as_nat h0 r * as_nat h0 f)
-
-let mul f r out =
+let scalar_bit #buf_type s n =
   let h0 = ST.get () in
-  BN.bn_mul #U64 4ul 4ul f r out;
-  let h1 = ST.get () in
-  SN.bn_mul_lemma (as_seq h0 f) (as_seq h0 r);
-  bignum_bn_v_is_as_nat h0 f;
-  bignum_bn_v_is_as_nat h0 r;
-  bignum_bn_v_is_wide_as_nat h1 out
+  mod_mask_lemma ((Lib.Sequence.index (as_seq h0 s) (v n / 8)) >>. (n %. 8ul)) 1ul;
+  assert_norm (1 = pow2 1 - 1);
+  assert (v (mod_mask #U8 #SEC 1ul) == v (u8 1));
+  to_u64 ((s.(n /. 8ul) >>. (n %. 8ul)) &. u8 1)
 
 
-val sq: f:felem -> out:widefelem -> Stack unit
-  (requires fun h ->
-    live h out /\ live h f /\ eq_or_disjoint f out)
-  (ensures  fun h0 _ h1 -> modifies (loc out) h0 h1 /\
-    wide_as_nat h1 out = as_nat h0 f * as_nat h0 f)
-
-let sq f out =
-  let h0 = ST.get () in
-  BN.bn_sqr #U64 4ul f out;
-  let h1 = ST.get () in
-  SN.bn_sqr_lemma (as_seq h0 f);
-  bignum_bn_v_is_as_nat h0 f;
-  bignum_bn_v_is_wide_as_nat h1 out
+let mul64 x y result temp =
+  let res = mul64_wide x y in
+  let l0, h0 = to_u64 res, to_u64 (res >>. 64ul) in
+  upd result (size 0) l0;
+  upd temp (size 0) h0
 
 
-val isZero_uint64_CT: f:felem -> Stack uint64
-  (requires fun h -> live h f)
-  (ensures fun h0 r h1 -> modifies0 h0 h1 /\
-    (if as_nat h0 f = 0 then uint_v r == pow2 64 - 1 else uint_v r == 0))
+///  Create zero and one
 
+let uploadZeroImpl f =
+  upd f (size 0) (u64 0);
+  upd f (size 1) (u64 0);
+  upd f (size 2) (u64 0);
+  upd f (size 3) (u64 0)
+
+
+let uploadOneImpl f =
+  upd f (size 0) (u64 1);
+  upd f (size 1) (u64 0);
+  upd f (size 2) (u64 0);
+  upd f (size 3) (u64 0)
+
+
+///  Comparison
+
+[@CInline]
 let isZero_uint64_CT f =
   let h0 = ST.get () in
   SN.bn_is_zero_mask_lemma (as_seq h0 f);
@@ -61,11 +57,7 @@ let isZero_uint64_CT f =
   BN.bn_is_zero_mask #U64 4ul f
 
 
-val compare_felem: a:felem -> b:felem -> Stack uint64
-  (requires fun h -> live h a /\ live h b)
-  (ensures fun h0 r h1 -> modifies0 h0 h1 /\
-    (if as_nat h0 a = as_nat h0 b then uint_v r == pow2 64 - 1 else uint_v r = 0))
-
+[@CInline]
 let compare_felem a b =
   let h0 = ST.get () in
   SN.bn_eq_mask_lemma (as_seq h0 a) (as_seq h0 b);
@@ -74,37 +66,22 @@ let compare_felem a b =
   BN.bn_eq_mask #U64 4ul a b
 
 
-// NOTE: changed precondition `eq_or_disjoint out x`
-val copy_conditional: out:felem -> x:felem
-  -> mask:uint64{uint_v mask = 0 \/ uint_v mask = pow2 64 - 1} -> Stack unit
-  (requires fun h -> live h out /\ live h x /\ eq_or_disjoint out x)
-  (ensures fun h0 _ h1 -> modifies (loc out) h0 h1 /\
-    (if uint_v mask = 0 then as_seq h1 out == as_seq h0 out else as_seq h1 out == as_seq h0 x))
+///  Conditional copy
 
+[@CInline]
 let copy_conditional out x mask =
   buf_mask_select x out mask out
 
 
-val cmovznz4: cin:uint64 -> x:felem -> y:felem -> out:felem -> Stack unit
-  (requires fun h ->
-    live h x /\ live h y /\ live h out /\
-    disjoint x out /\ eq_or_disjoint y out)
-  (ensures fun h0 _ h1 -> modifies1 out h0 h1 /\
-    (if uint_v cin = 0 then as_nat h1 out == as_nat h0 x else as_nat h1 out == as_nat h0 y))
-
+[@CInline]
 let cmovznz4 cin x y out =
   let mask = neq_mask cin (u64 0) in
   buf_mask_select y x mask out
 
 
-// NOTE: changed precondition `eq_or_disjoint x y`
-val add4: x:felem -> y:felem -> out:felem -> Stack uint64
-  (requires fun h ->
-    live h x /\ live h y /\ live h out /\
-    eq_or_disjoint x y /\ eq_or_disjoint x out /\ eq_or_disjoint y out)
-  (ensures fun h0 c h1 -> modifies (loc out) h0 h1 /\ v c <= 1 /\
-    as_nat h1 out + v c * pow2 256 == as_nat h0 x + as_nat h0 y)
+///  Addition and subtraction
 
+[@CInline]
 let add4 x y out =
   let h0 = ST.get () in
   let c = BN.bn_add_eq_len 4ul x y out in
@@ -116,34 +93,7 @@ let add4 x y out =
   c
 
 
-// NOTE: changed precondition `eq_or_disjoint x y`
-val add8: x:widefelem -> y:widefelem -> out:widefelem -> Stack uint64
-  (requires fun h ->
-    live h x /\ live h y /\ live h out /\
-    eq_or_disjoint x y /\ eq_or_disjoint x out /\ eq_or_disjoint y out)
-  (ensures fun h0 c h1 -> modifies (loc out) h0 h1 /\ v c <= 1 /\
-    wide_as_nat h1 out + v c * pow2 512 == wide_as_nat h0 x + wide_as_nat h0 y)
-
-let add8 x y out =
-  let h0 = ST.get () in
-  let c = BN.bn_add_eq_len 8ul x y out in
-  let h1 = ST.get () in
-  SN.bn_add_lemma (as_seq h0 x) (as_seq h0 y);
-  bignum_bn_v_is_wide_as_nat h0 x;
-  bignum_bn_v_is_wide_as_nat h0 y;
-  bignum_bn_v_is_wide_as_nat h1 out;
-  c
-
-
-val add4_variables: x:felem -> cin:uint64{uint_v cin <= 1}
-  -> y0:uint64 -> y1:uint64 -> y2:uint64 -> y3:uint64 -> result:felem ->
-  Stack uint64
-  (requires fun h -> live h x /\ live h result /\ eq_or_disjoint x result)
-  (ensures fun h0 c h1 -> modifies (loc result) h0 h1 /\ v c <= 1 /\
-    as_nat h1 result  + uint_v c * pow2 256 ==
-    as_nat h0 x + uint_v y0 + uint_v y1 * pow2 64 +
-    uint_v y2 * pow2 128 + uint_v y3 * pow2 192 + uint_v cin)
-
+[@CInline]
 let add4_variables x cin y0 y1 y2 y3 result =
     let h0 = ST.get() in
 
@@ -168,14 +118,31 @@ let add4_variables x cin y0 y1 y2 y3 result =
     cc
 
 
-val sub4_il: x:felem -> y:glbuffer uint64 (size 4) -> result:felem -> Stack uint64
-  (requires fun h ->
-    live h x /\ live h y /\ live h result /\
-    disjoint x result /\ disjoint result y)
-  (ensures fun h0 c h1 -> modifies1 result h0 h1 /\ v c <= 1 /\
-    as_nat h1 result - v c * pow2 256 == as_nat h0 x - as_nat_il h0 y /\
-    (if uint_v c = 0 then as_nat h0 x >= as_nat_il h0 y else as_nat h0 x < as_nat_il h0 y))
+[@CInline]
+let add8 x y out =
+  let h0 = ST.get () in
+  let c = BN.bn_add_eq_len 8ul x y out in
+  let h1 = ST.get () in
+  SN.bn_add_lemma (as_seq h0 x) (as_seq h0 y);
+  bignum_bn_v_is_wide_as_nat h0 x;
+  bignum_bn_v_is_wide_as_nat h0 y;
+  bignum_bn_v_is_wide_as_nat h1 out;
+  c
 
+
+[@CInline]
+let sub4 x y out =
+  let h0 = ST.get () in
+  let c = BN.bn_sub_eq_len 4ul x y out in
+  let h1 = ST.get () in
+  SN.bn_sub_lemma (as_seq h0 x) (as_seq h0 y);
+  bignum_bn_v_is_as_nat h0 x;
+  bignum_bn_v_is_as_nat h0 y;
+  bignum_bn_v_is_as_nat h1 out;
+  c
+
+
+[@CInline]
 let sub4_il x y result =
     let r0 = sub result (size 0) (size 1) in
     let r1 = sub result (size 1) (size 1) in
@@ -194,199 +161,27 @@ let sub4_il x y result =
     cc
 
 
-// NOTE: changed precondition `eq_or_disjoint x y`
-val sub4: x:felem -> y:felem -> out:felem -> Stack uint64
-  (requires fun h ->
-    live h x /\ live h y /\ live h out /\
-    eq_or_disjoint x y /\ eq_or_disjoint x out /\ eq_or_disjoint y out)
-  (ensures fun h0 c h1 -> modifies1 out h0 h1 /\ v c <= 1 /\
-    as_nat h1 out - v c * pow2 256 == as_nat h0 x - as_nat h0 y)
+///  Multiplication
 
-let sub4 x y out =
+[@CInline]
+let mul f r out =
   let h0 = ST.get () in
-  let c = BN.bn_sub_eq_len 4ul x y out in
+  BN.bn_mul #U64 4ul 4ul f r out;
   let h1 = ST.get () in
-  SN.bn_sub_lemma (as_seq h0 x) (as_seq h0 y);
-  bignum_bn_v_is_as_nat h0 x;
-  bignum_bn_v_is_as_nat h0 y;
-  bignum_bn_v_is_as_nat h1 out;
-  c
+  SN.bn_mul_lemma (as_seq h0 f) (as_seq h0 r);
+  bignum_bn_v_is_as_nat h0 f;
+  bignum_bn_v_is_as_nat h0 r;
+  bignum_bn_v_is_wide_as_nat h1 out
 
 
-// TODO: mv
-val mul64: x:uint64 -> y:uint64
-  -> result:lbuffer uint64 (size 1) -> temp:lbuffer uint64 (size 1) -> Stack unit
-  (requires fun h -> live h result /\ live h temp /\ disjoint result temp)
-  (ensures fun h0 _ h1 -> modifies (loc result |+| loc temp) h0 h1 /\ (
-    let h0 = Seq.index (as_seq h1 temp) 0 in
-    let result = Seq.index (as_seq h1 result) 0 in
-    uint_v result + uint_v h0 * pow2 64 = uint_v x * uint_v y))
-
-let mul64 x y result temp =
-  let res = mul64_wide x y in
-  let l0, h0 = to_u64 res, to_u64 (res >>. 64ul) in
-  upd result (size 0) l0;
-  upd temp (size 0) h0
-
-
-// local function
-val lemma_shift_256: a: int -> b: int -> c: int -> d: int -> Lemma (
-    a * pow2 64 * pow2 64 * pow2 64 * pow2 64 +
-    b * pow2 64 * pow2 64 * pow2 64 * pow2 64 * pow2 64 +
-    c * pow2 64 * pow2 64 * pow2 64 * pow2 64 * pow2 64 * pow2 64  +
-    d * pow2 64 * pow2 64 * pow2 64 * pow2 64 * pow2 64 * pow2 64 * pow2 64 ==
-    (a + b * pow2 64 + c * pow2 64 * pow2 64 + d * pow2 64 * pow2 64 * pow2 64) * pow2 64 * pow2 64 * pow2 64 * pow2 64)
-
-let lemma_shift_256 a b c d = ()
-
-
-// TODO: add bn_lshift
-val shift_256_impl: i:felem -> o:lbuffer uint64 (size 8) -> Stack unit
-  (requires fun h ->
-    live h i /\ live h o /\ disjoint i o)
-  (ensures fun h0 _ h1 -> modifies1 o h0 h1 /\
-    wide_as_nat h1 o == as_nat h0 i * pow2 256)
-
-let shift_256_impl i o =
-  assert_norm (pow2 64 * pow2 64 * pow2 64 * pow2 64 = pow2 256);
-
-  let h0 = ST.get() in
-    upd o (size 0) (u64 0);
-    upd o (size 1) (u64 0);
-    upd o (size 2) (u64 0);
-    upd o (size 3) (u64 0);
-    upd o (size 4) i.(size 0);
-    upd o (size 5) i.(size 1);
-    upd o (size 6) i.(size 2);
-    upd o (size 7) i.(size 3);
-
-  lemma_shift_256
-    (v (Lib.Sequence.index (as_seq h0 i) 0))
-    (v (Lib.Sequence.index (as_seq h0 i) 1))
-    (v (Lib.Sequence.index (as_seq h0 i) 2))
-    (v (Lib.Sequence.index (as_seq h0 i) 3))
-
-
-inline_for_extraction noextract
-val mod64: a:widefelem -> Stack uint64
-  (requires fun h -> live h a)
-  (ensures fun h0 r h1 -> modifies0 h0 h1 /\
-    wide_as_nat h1 a % pow2 64 = uint_v r)
-
-let mod64 a =
+[@CInline]
+let sq f out =
   let h0 = ST.get () in
-  let r = index a (size 0) in
-  bignum_bn_v_is_wide_as_nat h0 a;
-  Hacl.Spec.Bignum.Definitions.bn_eval_index (as_seq h0 a) 0;
-  assert (v r == wide_as_nat h0 a / pow2 0 % pow2 64);
-  r
-
-
-val shift8: t:widefelem -> out:widefelem -> Stack unit
-  (requires fun h ->
-    live h t /\ live h out /\ eq_or_disjoint t out)
-  (ensures fun h0 _ h1 -> modifies (loc out) h0 h1 /\
-    wide_as_nat h0 t / pow2 64 = wide_as_nat h1 out)
-
-let shift8 t out =
-  let t1 = index t (size 1) in
-  let t2 = index t (size 2) in
-  let t3 = index t (size 3) in
-  let t4 = index t (size 4) in
-  let t5 = index t (size 5) in
-  let t6 = index t (size 6) in
-  let t7 = index t (size 7) in
-
-  upd out (size 0) t1;
-  upd out (size 1) t2;
-  upd out (size 2) t3;
-  upd out (size 3) t4;
-  upd out (size 4) t5;
-  upd out (size 5) t6;
-  upd out (size 6) t7;
-  upd out (size 7) (u64 0)
-
-
-// TODO: mv
-inline_for_extraction noextract
-val scalar_bit:
-    #buf_type: buftype ->
-    s:lbuffer_t buf_type uint8 (size 32)
-  -> n:size_t{v n < 256}
-  -> Stack uint64
-    (requires fun h0 -> live h0 s)
-    (ensures  fun h0 r h1 -> h0 == h1 /\
-      r == Spec.ECDSA.ith_bit (as_seq h0 s) (v n) /\ v r <= 1)
-
-let scalar_bit #buf_type s n =
-  let h0 = ST.get () in
-  mod_mask_lemma ((Lib.Sequence.index (as_seq h0 s) (v n / 8)) >>. (n %. 8ul)) 1ul;
-  assert_norm (1 = pow2 1 - 1);
-  assert (v (mod_mask #U8 #SEC 1ul) == v (u8 1));
-  to_u64 ((s.(n /. 8ul) >>. (n %. 8ul)) &. u8 1)
-
-
-val uploadZeroImpl: f:felem -> Stack unit
-  (requires fun h -> live h f)
-  (ensures fun h0 _ h1 -> modifies (loc f) h0 h1 /\
-    as_nat h1 f == 0)
-
-let uploadZeroImpl f =
-  upd f (size 0) (u64 0);
-  upd f (size 1) (u64 0);
-  upd f (size 2) (u64 0);
-  upd f (size 3) (u64 0)
-
-
-val uploadOneImpl: f:felem -> Stack unit
-  (requires fun h -> live h f)
-  (ensures fun h0 _ h1 -> modifies (loc f) h0 h1 /\
-    as_nat h1 f == 1)
-
-let uploadOneImpl f =
-  upd f (size 0) (u64 1);
-  upd f (size 1) (u64 0);
-  upd f (size 2) (u64 0);
-  upd f (size 3) (u64 0)
-
-
-val toUint8: i:felem -> o:lbuffer uint8 (32ul) -> Stack unit
-  (requires fun h -> live h i /\ live h o /\ disjoint i o)
-  (ensures fun h0 _ h1 -> modifies (loc o) h0 h1 /\
-    as_seq h1 o == Lib.ByteSequence.uints_to_bytes_be #_ #_ #4 (as_seq h0 i))
-
-let toUint8 i o =
-  Lib.ByteBuffer.uints_to_bytes_be (size 4) o i
-
-
-val changeEndian: i:felem -> Stack unit
-  (requires fun h -> live h i)
-  (ensures  fun h0 _ h1 -> modifies1 i h0 h1 /\
-    as_seq h1 i == Spec.ECDSA.changeEndian (as_seq h0 i) /\
-    as_nat h1 i < pow2 256)
-
-let changeEndian i =
-  assert_norm (pow2 64 * pow2 64 = pow2 (2 * 64));
-  assert_norm (pow2 (2 * 64) * pow2 64 = pow2 (3 * 64));
-  assert_norm (pow2 (3 * 64) * pow2 64 = pow2 (4 * 64));
-  let zero = index i (size 0) in
-  let one = index i (size 1) in
-  let two = index i (size 2) in
-  let three = index i (size 3) in
-  upd i (size 0) three;
-  upd i (size 1) two;
-  upd i (size 2) one;
-  upd i (size 3) zero
-
-
-val toUint64ChangeEndian: i:lbuffer uint8 (size 32) -> o:felem -> Stack unit
-  (requires fun h -> live h i /\ live h o /\ disjoint i o)
-  (ensures  fun h0 _ h1 -> modifies (loc o) h0 h1 /\
-    as_seq h1 o == Spec.ECDSA.changeEndian (Lib.ByteSequence.uints_from_bytes_be (as_seq h0 i)))
-
-let toUint64ChangeEndian i o =
-  Lib.ByteBuffer.uints_from_bytes_be o i;
-  changeEndian o
+  BN.bn_sqr #U64 4ul f out;
+  let h1 = ST.get () in
+  SN.bn_sqr_lemma (as_seq h0 f);
+  bignum_bn_v_is_as_nat h0 f;
+  bignum_bn_v_is_wide_as_nat h1 out
 
 
 // local function
@@ -471,14 +266,7 @@ let mul1_il f u result =
   c3 +! temp0
 
 
-inline_for_extraction noextract
-val shortened_mul: a:glbuffer uint64 (size 4) -> b:uint64 -> result:widefelem -> Stack unit
-  (requires fun h ->
-    live h a /\ live h result /\ wide_as_nat h result = 0)
-  (ensures fun h0 _ h1 -> modifies (loc result) h0 h1 /\
-    as_nat_il h0 a * uint_v b = wide_as_nat h1 result /\
-    wide_as_nat h1 result < pow2 320)
-
+[@CInline]
 let shortened_mul a b result =
   let result04 = sub result (size 0) (size 4) in
   let result48 = sub result (size 4) (size 4) in
@@ -491,3 +279,92 @@ let shortened_mul a b result =
     assert(Lib.Sequence.index (as_seq h0 result) 7 == Lib.Sequence.index (as_seq h0 result48) 3);
 
     assert_norm( pow2 64 * pow2 64 * pow2 64 * pow2 64 = pow2 256)
+
+
+///  pow2-operations
+
+// local function
+val lemma_shift_256: a: int -> b: int -> c: int -> d: int -> Lemma (
+    a * pow2 64 * pow2 64 * pow2 64 * pow2 64 +
+    b * pow2 64 * pow2 64 * pow2 64 * pow2 64 * pow2 64 +
+    c * pow2 64 * pow2 64 * pow2 64 * pow2 64 * pow2 64 * pow2 64  +
+    d * pow2 64 * pow2 64 * pow2 64 * pow2 64 * pow2 64 * pow2 64 * pow2 64 ==
+    (a + b * pow2 64 + c * pow2 64 * pow2 64 + d * pow2 64 * pow2 64 * pow2 64) * pow2 64 * pow2 64 * pow2 64 * pow2 64)
+
+let lemma_shift_256 a b c d = ()
+
+
+[@CInline]
+let shift_256_impl i o =
+  assert_norm (pow2 64 * pow2 64 * pow2 64 * pow2 64 = pow2 256);
+
+  let h0 = ST.get() in
+    upd o (size 0) (u64 0);
+    upd o (size 1) (u64 0);
+    upd o (size 2) (u64 0);
+    upd o (size 3) (u64 0);
+    upd o (size 4) i.(size 0);
+    upd o (size 5) i.(size 1);
+    upd o (size 6) i.(size 2);
+    upd o (size 7) i.(size 3);
+
+  lemma_shift_256
+    (v (Lib.Sequence.index (as_seq h0 i) 0))
+    (v (Lib.Sequence.index (as_seq h0 i) 1))
+    (v (Lib.Sequence.index (as_seq h0 i) 2))
+    (v (Lib.Sequence.index (as_seq h0 i) 3))
+
+
+[@CInline]
+let shift8 t out =
+  let t1 = index t (size 1) in
+  let t2 = index t (size 2) in
+  let t3 = index t (size 3) in
+  let t4 = index t (size 4) in
+  let t5 = index t (size 5) in
+  let t6 = index t (size 6) in
+  let t7 = index t (size 7) in
+
+  upd out (size 0) t1;
+  upd out (size 1) t2;
+  upd out (size 2) t3;
+  upd out (size 3) t4;
+  upd out (size 4) t5;
+  upd out (size 5) t6;
+  upd out (size 6) t7;
+  upd out (size 7) (u64 0)
+
+
+let mod64 a =
+  let h0 = ST.get () in
+  bignum_bn_v_is_wide_as_nat h0 a;
+  Hacl.Spec.Bignum.Definitions.bn_eval_index (as_seq h0 a) 0;
+  assert (v (Lib.Sequence.index (as_seq h0 a) 0) == wide_as_nat h0 a / pow2 0 % pow2 64);
+  index a (size 0)
+
+
+///  Conversion between bignum and bytes representation
+
+[@CInline]
+let toUint8 i o =
+  Lib.ByteBuffer.uints_to_bytes_be (size 4) o i
+
+
+let changeEndian i =
+  assert_norm (pow2 64 * pow2 64 = pow2 (2 * 64));
+  assert_norm (pow2 (2 * 64) * pow2 64 = pow2 (3 * 64));
+  assert_norm (pow2 (3 * 64) * pow2 64 = pow2 (4 * 64));
+  let zero = index i (size 0) in
+  let one = index i (size 1) in
+  let two = index i (size 2) in
+  let three = index i (size 3) in
+  upd i (size 0) three;
+  upd i (size 1) two;
+  upd i (size 2) one;
+  upd i (size 3) zero
+
+
+[@CInline]
+let toUint64ChangeEndian i o =
+  Lib.ByteBuffer.uints_from_bytes_be o i;
+  changeEndian o
